***NO_CI*** cleaning up hyperstack and hyperheap, simplified many definitions and trying so that client don't have to open/use hyperheaps at all

ulib/FStar.HyperHeap.fst
@@ -16,4 +16,4 @@
 module FStar.HyperHeap
 
 include FStar.Monotonic.HyperHeap
-type rref (id:rid) (a:Type) = mrref id a (FStar.Heap.trivial_preorder a)
+type rref (id:hh_rid) (a:Type) = mrref id a (FStar.Heap.trivial_preorder a)
